Make copy functions type-generic

vale/code/arch/x64/interop/Fast_stdcalls.fst
@@ -165,96 +165,8 @@ let fast_add1
   let x, _ = lowstar_add1_normal_t out f1 f2 () in
   x
   
-let rec ghost_copy64_8 (b:u256) (b8:b8{B.length b8 == 32}) 
-  (h0:HS.mem{B.live h0 b /\ B.live h0 b8}) 
-  (h_accu:HS.mem{B.live h_accu b /\ B.live h_accu b8 /\ 
-    FStar.HyperStack.ST.equal_domains h0 h_accu /\
-    B.modifies (B.loc_buffer b8) h0 h_accu})
-  (i:nat{i <= 4}) : 
-  Ghost (x:HS.mem{FStar.HyperStack.ST.equal_domains h0 x})
-  (requires (forall (j:nat{j < i}). 
-    Seq.index (B.as_seq h0 b) j == low_buffer_read TUInt64 h_accu b8 j))
-  (ensures fun h1 ->
-    B.live h1 b /\ B.live h1 b8 /\
-    B.modifies (B.loc_buffer b8) h0 h1 /\
-    (forall (j:nat{j < 4}). {:pattern low_buffer_read TUInt64 h1 b8 j} Seq.index (B.as_seq h0 b) j == low_buffer_read TUInt64 h1 b8 j))
-   (decreases %[4 - i])
-  =
-  if i >= 4 then h_accu
-  else
-    let bv = BV.mk_buffer_view b8 Views.view64 in
-    let v = Seq.index (B.as_seq h0 b) i in
-    BV.as_buffer_mk_buffer_view b8 Views.view64;
-    BV.get_view_mk_buffer_view b8 Views.view64;
-    BV.length_eq bv;      
-    BV.upd_equal_domains h_accu bv i v;
-    BV.upd_modifies h_accu bv i v;
-    let h1 = BV.upd h_accu bv i v in
-    let aux (j:nat{j <= i}) : Lemma
-      (Seq.index (B.as_seq h0 b) j == low_buffer_read TUInt64 h1 b8 j) =
-      BV.sel_upd bv i j v h_accu
-    in Classical.forall_intro aux;  
-    ghost_copy64_8 b b8 h0 h1 (i+1)
+open Vale.Interop.Cast
 
-
-let copy64_8 (b:u256) (b8:b8{B.length b8 == 32}) : Stack unit
-  (requires fun h -> B.live h b /\ B.live h b8)
-  (ensures fun h0 _ h -> 
-    B.live h b /\ B.live h b8 /\ 
-    B.modifies (B.loc_buffer b8) h0 h /\
-    (forall (i:nat{i < 4}). {:pattern low_buffer_read TUInt64 h b8 i} Seq.index (B.as_seq h0 b) i == low_buffer_read TUInt64 h b8 i)) =
-    IA.st_put (fun h0 -> B.live h0 b /\ B.live h0 b8) (fun h0 -> (), ghost_copy64_8 b b8 h0 h0 0)
-
-
-let ghost_copy8_64 (b:u256) (b8:b8{B.length b8 == 32})
-  (h0:HS.mem{B.live h0 b /\ B.live h0 b8})
-  : Ghost  (x:HS.mem{FStar.HyperStack.ST.equal_domains h0 x})
-  (requires True)
-  (ensures fun h1 ->
-    B.live h1 b /\ B.live h1 b8 /\
-    B.modifies (B.loc_buffer b) h0 h1 /\
-    (forall (j:nat{j < 4}). Seq.index (B.as_seq h1 b) j == low_buffer_read TUInt64 h0 b8 j)) 
-  = let bv = BV.mk_buffer_view b8 Views.view64 in
-    let s = BV.as_seq h0 bv in
-    BV.as_buffer_mk_buffer_view b8 Views.view64;
-    BV.get_view_mk_buffer_view b8 Views.view64;
-    BV.length_eq bv;
-    B.g_upd_seq_as_seq b s h0;
-    Classical.forall_intro (BV.as_seq_sel h0 bv);
-    B.g_upd_seq b s h0
-
-let imm_ghost_copy8_64 (b:u256) (b8:b8{B.length b8 == 32})
-  (h0:HS.mem{B.live h0 b /\ B.live h0 b8 /\
-    (forall (j:nat{j < 4}). Seq.index (B.as_seq h0 b) j == low_buffer_read TUInt64 h0 b8 j)})
-  : Ghost  (x:HS.mem{FStar.HyperStack.ST.equal_domains h0 x})
-  (requires True)
-  (ensures fun h1 -> h1 == h0)
-  = let bv = BV.mk_buffer_view b8 Views.view64 in
-    let s = BV.as_seq h0 bv in
-    BV.as_buffer_mk_buffer_view b8 Views.view64;
-    BV.get_view_mk_buffer_view b8 Views.view64;
-    BV.length_eq bv;
-    B.g_upd_seq_as_seq b s h0;
-    Classical.forall_intro (BV.as_seq_sel h0 bv);
-    assert (Seq.equal (B.as_seq h0 b) (BV.as_seq h0 bv));
-    B.lemma_g_upd_with_same_seq b h0;
-    B.g_upd_seq b s h0
-
-
-let copy8_64 (b:u256) (b8:b8{B.length b8 == 32}) : Stack unit
-  (requires fun h -> B.live h b /\ B.live h b8)
-  (ensures fun h0 _ h1 -> B.live h1 b /\ B.live h0 b8 /\ B.modifies (B.loc_buffer b) h0 h1 /\
-    (forall (i:nat{i < 4}). Seq.index (B.as_seq h1 b) i == low_buffer_read TUInt64 h0 b8 i))
-  = IA.st_put (fun h0 -> B.live h0 b /\ B.live h0 b8) (fun h0 -> (), ghost_copy8_64 b b8 h0)
-
-let imm_copy8_64 (b:u256) (b8:b8{B.length b8 == 32}) : Stack unit
-  (requires fun h -> B.live h b /\ B.live h b8 /\
-    (forall (i:nat{i < 4}). Seq.index (B.as_seq h b) i == low_buffer_read TUInt64 h b8 i))
-  (ensures fun h0 _ h -> h0 == h) 
-  = IA.st_put 
-    (fun h0 -> B.live h0 b /\ B.live h0 b8 /\ (forall (j:nat{j < 4}). Seq.index (B.as_seq h0 b) j == low_buffer_read TUInt64 h0 b8 j))
-    (fun h0 -> (), imm_ghost_copy8_64 b b8 h0)
-  
 
 let fast_add1_alloca
   (out64:u256)
@@ -284,11 +196,11 @@ let fast_add1_alloca
       (B.loc_union (B.loc_buffer out64) (B.loc_buffer f1))
       (B.loc_buffer out)) h0 h1 /\
     as_nat out64 h1 + pow2_256 `op_Multiply` UInt64.v c == as_nat f164 h0 + UInt64.v f2)
-  = copy64_8 out64 out;
-    copy64_8 f164 f1;
+  = copy_down out64 out;
+    copy_down f164 f1;
     let x = fast_add1 out f1 f2 in
-    imm_copy8_64 f164 f1;
-    copy8_64 out64 out;
+    imm_copy_up f164 f1;
+    copy_up out64 out;
     x
 
 let add1
