vale/code/arch/x64/interop/Vale.Interop.Cast.fst
@@ -1,0 +1,100 @@
+module Vale.Interop.Cast
+
+module B = LowStar.Buffer
+module BV = LowStar.BufferView
+module HS = FStar.HyperStack
+open FStar.HyperStack.ST
+
+open Interop.Base
+module IA = Interop.Assumptions
+open Vale.AsLowStar.MemoryHelpers
+module LSig = Vale.AsLowStar.LowStarSig
+
+open FStar.Mul
+
+
+let rec ghost_copy_down (#t:base_typ) (b:b_t t) (b8:b_t TUInt8{B.length b8 == B.length b * view_n t}) 
+  (h0:HS.mem{B.live h0 b /\ B.live h0 b8}) 
+  (h_accu:HS.mem{B.live h_accu b /\ B.live h_accu b8 /\ 
+    equal_domains h0 h_accu /\
+    B.modifies (B.loc_buffer b8) h0 h_accu})
+  (n:nat{B.length b == n})
+  (i:nat{i <= n}) : 
+  Ghost (x:HS.mem{equal_domains h0 x})
+  (requires (forall (j:nat{j < i}). 
+    Seq.index (B.as_seq h0 b) j == low_buffer_read t h_accu b8 j))
+  (ensures fun h1 ->
+    B.live h1 b /\ B.live h1 b8 /\
+    B.modifies (B.loc_buffer b8) h0 h1 /\
+    (forall (j:nat{j < n}). {:pattern low_buffer_read t h1 b8 j} Seq.index (B.as_seq h0 b) j == low_buffer_read t h1 b8 j))
+   (decreases %[n - i])
+  =
+  if i >= n then h_accu
+  else
+    let view = LSig.view_of_base_typ t in
+    let bv = BV.mk_buffer_view b8 view in
+    let v = Seq.index (B.as_seq h0 b) i in
+    BV.as_buffer_mk_buffer_view b8 view;
+    BV.get_view_mk_buffer_view b8 view;
+    BV.length_eq bv;      
+    BV.upd_equal_domains h_accu bv i v;
+    BV.upd_modifies h_accu bv i v;
+    let h1 = BV.upd h_accu bv i v in
+    let aux (j:nat{j <= i}) : Lemma
+      (Seq.index (B.as_seq h0 b) j == low_buffer_read t h1 b8 j) =
+      BV.sel_upd bv i j v h_accu
+    in Classical.forall_intro aux;  
+    ghost_copy_down b b8 h0 h1 n (i+1)
+
+
+let copy_down #t b b8 =
+    IA.st_put 
+      (fun h0 -> B.live h0 b /\ B.live h0 b8) 
+      (fun h0 -> (), ghost_copy_down b b8 h0 h0 (B.length b) 0)
+
+let ghost_copy_up (#t:base_typ) (b:b_t t) (b8:b_t TUInt8{B.length b8 == B.length b * view_n t})
+  (h0:HS.mem{B.live h0 b /\ B.live h0 b8})
+  : Ghost (x:HS.mem{equal_domains h0 x})
+  (requires True)
+  (ensures fun h1 ->
+    B.live h1 b /\ B.live h1 b8 /\
+    B.modifies (B.loc_buffer b) h0 h1 /\
+    (forall (j:nat{j < B.length b}). Seq.index (B.as_seq h1 b) j == low_buffer_read t h0 b8 j)) 
+  = let view = LSig.view_of_base_typ t in
+    let bv = BV.mk_buffer_view b8 view in
+    let s = BV.as_seq h0 bv in
+    BV.as_buffer_mk_buffer_view b8 view;
+    BV.get_view_mk_buffer_view b8 view;
+    BV.length_eq bv;
+    B.g_upd_seq_as_seq b s h0;
+    Classical.forall_intro (BV.as_seq_sel h0 bv);
+    B.g_upd_seq b s h0
+
+let imm_ghost_copy_up (#t:base_typ) (b:b_t t) (b8:b_t TUInt8{B.length b8 == B.length b * view_n t})
+  (h0:HS.mem{B.live h0 b /\ B.live h0 b8 /\
+    (forall (j:nat{j < B.length b}). Seq.index (B.as_seq h0 b) j == low_buffer_read t h0 b8 j)})
+  : Ghost  (x:HS.mem{equal_domains h0 x})
+  (requires True)
+  (ensures fun h1 -> h1 == h0)
+  = let view = LSig.view_of_base_typ t in
+    let bv = BV.mk_buffer_view b8 view in
+    let s = BV.as_seq h0 bv in
+    BV.as_buffer_mk_buffer_view b8 view;
+    BV.get_view_mk_buffer_view b8 view;
+    BV.length_eq bv;
+    B.g_upd_seq_as_seq b s h0;
+    Classical.forall_intro (BV.as_seq_sel h0 bv);
+    assert (Seq.equal (B.as_seq h0 b) (BV.as_seq h0 bv));
+    B.lemma_g_upd_with_same_seq b h0;
+    B.g_upd_seq b s h0
+
+
+let copy_up #t b b8
+  = IA.st_put (fun h0 -> B.live h0 b /\ B.live h0 b8) (fun h0 -> (), ghost_copy_up b b8 h0)
+
+let imm_copy_up #t b b8
+  = IA.st_put 
+    (fun h0 -> B.live h0 b /\ B.live h0 b8 /\ 
+      (forall (j:nat{j < B.length b}). Seq.index (B.as_seq h0 b) j == low_buffer_read t h0 b8 j))
+    (fun h0 -> (), imm_ghost_copy_up b b8 h0)
+
