vale/code/arch/x64/interop/Vale.Interop.Cast.fsti
@@ -1,0 +1,32 @@
+module Vale.Interop.Cast
+
+module B = LowStar.Buffer
+module BV = LowStar.BufferView
+module HS = FStar.HyperStack
+open FStar.HyperStack.ST
+
+open Interop.Base
+open Vale.AsLowStar.MemoryHelpers
+
+open FStar.Mul
+
+unfold
+let b_t (t:base_typ) = b:B.buffer (base_typ_as_type t)
+
+val copy_down (#t:base_typ) (b:b_t t) (b8:b_t TUInt8) : Stack unit
+  (requires fun h -> B.live h b /\ B.live h b8 /\ B.length b8 == B.length b * view_n t)
+  (ensures fun h0 _ h -> 
+    B.live h b /\ B.live h b8 /\ 
+    B.modifies (B.loc_buffer b8) h0 h /\
+    (forall (i:nat{i < B.length b}). {:pattern low_buffer_read t h b8 i} Seq.index (B.as_seq h0 b) i == low_buffer_read t h b8 i))
+
+val copy_up (#t:base_typ) (b:b_t t) (b8:b_t TUInt8) : Stack unit
+  (requires fun h -> B.live h b /\ B.live h b8 /\ B.length b8 == B.length b * view_n t)
+  (ensures fun h0 _ h1 -> 
+    B.live h1 b /\ B.live h0 b8 /\ B.modifies (B.loc_buffer b) h0 h1 /\
+    (forall (i:nat{i < B.length b}). Seq.index (B.as_seq h1 b) i == low_buffer_read t h0 b8 i))
+
+val imm_copy_up (#t:base_typ) (b:b_t t) (b8:b_t TUInt8) : Stack unit
+  (requires fun h -> B.live h b /\ B.live h b8 /\ B.length b8 == B.length b * view_n t /\
+    (forall (i:nat{i < B.length b}). Seq.index (B.as_seq h b) i == low_buffer_read t h b8 i))
+  (ensures fun h0 _ h -> h0 == h) 
